examples/dev/sw/IR.sml
@@ -1,13 +1,11 @@
 structure IR =
 struct
 
-
-open HolKernel Parse boolLib wordsTheory wordsLib pairLib
+open HolKernel Parse boolLib wordsTheory pairLib
      numSyntax
 
 val w32 = Type `:word32`;
 val n2w_tm = Term `n2w:num -> word32`;
-
 
 fun is_binop op1 =
   if not (is_comb op1) then false
@@ -23,12 +21,15 @@ fun is_binop op1 =
                         oper_name = "/" orelse
                         oper_name = "&&" orelse
                         oper_name = "!!" orelse
-                        oper_name = "??" orelse
                         oper_name = "<<" orelse
                         oper_name = ">>" orelse
                         oper_name = ">>#" orelse
-     			oper_name = ">>>" orelse
-     			  oper_name = "word_add" orelse
+			oper_name = ">>>" orelse
+			oper_name = "??" orelse
+            oper_name = "word_or" orelse
+            oper_name = "word_and" orelse
+            oper_name = "word_xor" orelse
+            oper_name = "word_add" orelse
       			oper_name = "word_sub" orelse
       			oper_name = "word_mul" orelse
       			oper_name = "bitwise_and" orelse
@@ -36,10 +37,7 @@ fun is_binop op1 =
       			oper_name = "word_lsl" orelse
       			oper_name = "word_lsr" orelse
       			oper_name = "word_asr" orelse
-            oper_name = "word_ror" orelse
-            oper_name = "word_and" orelse
-            oper_name = "word_or" orelse
-            oper_name = "word_xor" orelse
+      			oper_name = "word_ror" orelse
       			oper_name = "bitwise_eor"
                         then true
                 else false
@@ -77,12 +75,12 @@ fun convert_binop bop =
       else if oper_name = "-" then Tree.MINUS
       else if oper_name = "*" then Tree.MUL
       else if oper_name = "/" then Tree.DIV
+      else if oper_name = "&&" then Tree.AND
+      else if oper_name = "!!" then Tree.OR
       else if oper_name = "<<" then Tree.LSHIFT
       else if oper_name = ">>" then Tree.RSHIFT
       else if oper_name = ">>#" then Tree.ARSHIFT
       else if oper_name = ">>>" then Tree.ROR
-      else if oper_name = "&&" then Tree.AND
-      else if oper_name = "||" then Tree.OR
       else if oper_name = "??" then Tree.XOR
 
       else if oper_name = "word_and" then Tree.AND
@@ -159,7 +157,6 @@ fun mk_MOVE e1 (Tree.ESEQ(s1, Tree.ESEQ(s2,e2))) =
 	Tree.PAIR(mk_PAIR e1, mk_PAIR e2)
   |  mk_PAIR exp =
 	  Tree.TEMP (inspectVar(Temp.makestring(Temp.newtemp())))  
-val exp = rhs
 
  fun analyzeExp exp =
 
@@ -180,7 +177,7 @@ val exp = rhs
       	        Tree.TEMP (inspectVar v)
             end
 	else
-      Tree.NCONST Arbint.zero
+	    Tree.NCONST Arbint.zero
 
      else if is_cond exp then
         let val (c,t,f) = dest_cond exp;
