examples/dev/sw/rulesScript.sml
@@ -1,3 +1,14 @@
+(* interactive use:
+
+quietdec := true;
+loadPath := (concat Globals.HOLDIR "/examples/dev/sw") :: !loadPath;
+
+app load ["numLib", "relationTheory", "arithmeticTheory", "preARMTheory", "pairTheory",
+     "pred_setSimps", "pred_setTheory", "listTheory", "rich_listTheory", "whileTheory", "ARMCompositionTheory", "ILTheory"];
+
+quietdec := false;
+*)
+
 
 open HolKernel Parse boolLib bossLib numLib relationTheory arithmeticTheory preARMTheory pairTheory
      pred_setSimps pred_setTheory listTheory rich_listTheory whileTheory ARMCompositionTheory ILTheory;
@@ -20,21 +31,30 @@ val _ = Globals.priming := NONE;
 (*---------------------------------------------------------------------------------*)
 (*      read from an data state                                                    *) 
 (*---------------------------------------------------------------------------------*)
+val _ = Hol_datatype `
+    REXP = RR of MREG          
+         | RM of MMEM          
+         | RC of DATA          
+    `;
+
 
 val mread_def = Define `
-    (mread st mexp = read st (toEXP mexp))`;
+     (mread st (RR r) = read st (toREG r)) /\
+     (mread st (RM m) = read st (toMEM m)) /\
+     (mread st (RC c) = c)`;
 
-val mread_thm = store_thm ("mread_thm",
-        ``(!st r. mread st (MR r) = read st (toREG r)) /\
-          (!st s c. mread st (MC s c) = read st (WCONST (w2w c #>> (2 * w2n s))))``,
-
-        SIMP_TAC std_ss [mread_def, toEXP_def]);
-
-       
 val _ = add_rule {term_name = "mread", fixity = Suffix 60,
 		  pp_elements = [TOK "<", TM, TOK ">"],
                   paren_style = OnlyIfNecessary,
                   block_style = (AroundSameName, (PP.INCONSISTENT, 0))} handle HOL_ERR e => print (#message e);
+
+
+(*---------------------------------------------------------------------------------*)
+(*      The fp and sp point to the default positions                               *)
+(*---------------------------------------------------------------------------------*)
+
+val proper_def = Define `
+    proper = (\(regs,mem):DSTATE. (regs ' 11 = 100w) /\ (regs ' 13 = 100w))`;
 
 
 (*---------------------------------------------------------------------------------*)
@@ -126,7 +146,7 @@ val BLK_RULE = Q.store_thm (
 val CJ_RULE = Q.store_thm (
    "CJ_RULE",
    `!P Q cond ir1 ir2 st. WELL_FORMED ir1 /\ WELL_FORMED ir2 /\
-      HSPEC (\st.eval_cond cond st /\ P st) ir1 Q /\ HSPEC (\st.~eval_cond cond st /\ P st) ir2 Q ==> 
+      HSPEC (\st.eval_il_cond cond st /\ P st) ir1 Q /\ HSPEC (\st.~eval_il_cond cond st /\ P st) ir2 Q ==> 
       HSPEC P (CJ cond ir1 ir2) Q`,
     RW_TAC std_ss [HSPEC_def] THEN 
     METIS_TAC [IR_SEMANTICS_CJ]
@@ -149,7 +169,7 @@ val CJ_RULE_2 = Q.store_thm (
 val TR_RULE = Q.store_thm (
    "TR_RULE",
    `!cond ir P Q.
-        WELL_FORMED ir /\  WF_TR (cond, translate ir) /\
+        WELL_FORMED ir /\  WF_TR (translate_condition cond, translate ir) /\
            HSPEC P ir P ==> HSPEC P (TR cond ir) P`,
    RW_TAC std_ss [HSPEC_def] THEN
    METIS_TAC [HOARE_TR_IR]
@@ -168,12 +188,12 @@ val WF_DEF_2 = Q.store_thm (
 val WF_TR_LEM_1 = Q.store_thm (
    "WF_TR_LEM_1",
    `!cond ir st. WELL_FORMED ir /\
-           WF (\st1 st0. ~eval_cond cond st0 /\ (st1 = run_ir ir st0)) ==>
-           WF_TR (cond,translate ir)`,
+           WF (\st1 st0. ~eval_il_cond cond st0 /\ (st1 = run_ir ir st0)) ==>
+           WF_TR (translate_condition cond,translate ir)`,
    
    RW_TAC std_ss [WELL_FORMED_def, WF_TR_def, WF_Loop_def, run_ir_def, run_arm_def] THEN
    POP_ASSUM MP_TAC THEN Q.ABBREV_TAC `arm = translate ir` THEN STRIP_TAC THEN
-   Q.EXISTS_TAC `\s1 s0. if eval_cond cond (get_st s0) then F else (get_st s1 = get_st (runTo (upload arm (\i. ARB) (FST (FST s0))) 
+   Q.EXISTS_TAC `\s1 s0. if eval_il_cond cond (get_st s0) then F else (get_st s1 = get_st (runTo (upload arm (\i. ARB) (FST (FST s0))) 
              (FST (FST s0) + LENGTH (translate ir)) s0))` THEN
    STRIP_TAC THENL [
       FULL_SIMP_TAC std_ss [WF_DEF_2, GSYM RIGHT_FORALL_IMP_THM] THEN
@@ -190,7 +210,7 @@ val WF_TR_LEM_1 = Q.store_thm (
               METIS_TAC [well_formed_def, get_st_def, DSTATE_IRRELEVANT_PCS, status_independent_def, FST, DECIDE (Term `!x.0 + x = x`)] THEN
           METIS_TAC [FST,SND,get_st_def, ABS_PAIR_THM],
 
-      RW_TAC std_ss [get_st_def] THEN
+      RW_TAC std_ss [get_st_def, eval_il_cond_def] THEN
           METIS_TAC [WELL_FORMED_INSTB]
       ]
    );
@@ -198,9 +218,9 @@ val WF_TR_LEM_1 = Q.store_thm (
 val WF_TR_LEM_2 = Q.store_thm (
    "WF_TR_LEM_2",
     `!cond ir prj_f f cond_f.
-        (!st. cond_f (prj_f st) = eval_cond cond st) /\ (!st. prj_f (run_ir ir st) = f (prj_f st)) /\ 
+        (!st. cond_f (prj_f st) = eval_il_cond cond st) /\ (!st. prj_f (run_ir ir st) = f (prj_f st)) /\ 
         WF (\t1 t0. ~cond_f t0 /\ (t1 = f t0)) ==>
-           WF (\st1 st0. ~eval_cond cond st0 /\ (st1 = run_ir ir st0))`,
+           WF (\st1 st0. ~eval_il_cond cond st0 /\ (st1 = run_ir ir st0))`,
 
    RW_TAC std_ss [WF_DEF_2] THEN
    Q.PAT_ASSUM `!P.p` (ASSUME_TAC o Q.SPEC `\t:'a. ?y:DSTATE. (prj_f y = t) /\ P y`) THEN
@@ -224,169 +244,370 @@ val WF_TR_LEM_3 = Q.store_thm (
    RW_TAC std_ss []
    );
 
+val WF_TR_THM_1 = Q.store_thm (
+   "WF_TR_THM_1",
+    `!cond ir prj_f f cond_f pre_p.
+        (!st. cond_f (prj_f st) = eval_il_cond cond st) /\
+        (!st. pre_p st ==> (prj_f (run_ir ir st) = f (prj_f st))) /\
+        WF (\t1 t0. ~cond_f t0 /\ (t1 = f t0)) ==>
+           WF (\st1 st0. (pre_p st0) /\ ~(eval_il_cond cond st0) /\ (st1 = run_ir ir st0))`,
+
+   RW_TAC std_ss [WF_DEF_2] THEN
+   Q.PAT_ASSUM `!P.p` (ASSUME_TAC o Q.SPEC `\t:'a. ?y:DSTATE. (prj_f y = t) /\ P y`) THEN
+   FULL_SIMP_TAC std_ss [GSYM RIGHT_EXISTS_IMP_THM] THEN
+   RES_TAC THEN
+   Q.EXISTS_TAC `y` THEN
+   RW_TAC std_ss [] THEN
+   `~cond_f (prj_f y)` by METIS_TAC [] THEN
+   RES_TAC THEN
+   Q.PAT_ASSUM `!y1.p` (ASSUME_TAC o Q.SPEC `prj_f (run_ir ir y)`) THEN
+   METIS_TAC []
+  );
+
 (*---------------------------------------------------------------------------------*)
-(*      Hoare Rules on Projection on Inputs and Ouputs                             *)
+(*      Hoare Rules on Projection on Inputs and Ouputs (represented                *)
+(*                    by projective functions                                      *)
 (*      The pre-conditions and post-conditions (on data other than inputs and      *)
 (*        outputs) are also specified                                              *) 
 (*---------------------------------------------------------------------------------*)
 
 val PSPEC_def = Define `
-    PSPEC ir (pre_p,post_p) (in_f,f,out_f) = !v. HSPEC (\st. (in_f st = v) /\ pre_p st) ir (\st. (out_f st = f v) /\ post_p st)`;
+    PSPEC ir (pre_p,post_p) stk_f (in_f,f,out_f) = 
+        !v x. HSPEC (\st. pre_p st /\ (stk_f st = x) /\ (in_f st = v))
+                 ir (\st. post_p st /\ (stk_f st = x) /\ (out_f st = f v))`;
 
 val _ = type_abbrev("PSPEC_TYPE", type_of (Term `PSPEC`));
 
-val PROJ_POST_RULE = Q.store_thm (
-   "PROJ_POST_RULE",
-   `!ir in_f out_f convert_f.
-     PSPEC ir (pre_p,post_p) (in_f,f,out_f) 
+val PSPEC_STACK = Q.store_thm (
+   "PSPEC_STACK",
+   `!ir pre_p post_p stk_f in_f f out_f x.
+     PSPEC ir (pre_p,post_p) stk_f (in_f,f,out_f) 
        ==>
-       PSPEC ir (pre_p, post_p) (in_f, convert_f o f, convert_f o out_f)`,
+       HSPEC (\st. pre_p st /\ (stk_f st = x)) ir (\st. post_p st /\ (stk_f st = x))`,
      RW_TAC std_ss [PSPEC_def, HSPEC_def]
    );
 
-val PROJ_SC_RULE = Q.store_thm (
-   "PROJ_SC_RULE",
-   `!ir1 ir2 f1 f2 pre_p1 post_p1 post_p2 in_f1 out_f1 out_f2.
-     WELL_FORMED ir1 /\ WELL_FORMED ir2 /\
-     PSPEC ir1 (pre_p1,post_p1) (in_f1,f1,out_f1) /\ PSPEC ir2 (post_p1,post_p2) (out_f1,f2,out_f2) 
+val PSPEC_CHARACTERISTIC = Q.store_thm (
+   "PSPEC_CHARACTERISTIC",
+   `!ir pre_p post_p stk_f in_f f out_f.
+     PSPEC ir (pre_p,post_p) stk_f (in_f,f,out_f) 
        ==>
-       PSPEC (SC ir1 ir2) (pre_p1,post_p2) (in_f1,f2 o f1,out_f2)`,
+       HSPEC (\st. pre_p st /\ (in_f st = v)) ir (\st. post_p st /\ (out_f st = f v))`,
+     RW_TAC std_ss [PSPEC_def, HSPEC_def]
+   );
+
+val PRJ_SHUFFLE_RULE = Q.store_thm (
+   "PRJ_SHUFFLE_RULE",
+   `!ir pre_p post_p stk_f in_f f out_f shuffle_f.
+     PSPEC ir (pre_p,post_p) stk_f (in_f,f,out_f) 
+       ==>
+       PSPEC ir (pre_p, post_p) stk_f (in_f, shuffle_f o f, shuffle_f o out_f)`,
+     RW_TAC std_ss [PSPEC_def, HSPEC_def]
+   );
+
+val PRJ_SHUFFLE_RULE2 = Q.store_thm (
+   "PRJ_SHUFFLE_RULE2",
+   `!ir pre_p post_p stk_f in_f f out_f g in_f'.
+     PSPEC ir (pre_p, post_p) stk_f (in_f, f, out_f) /\ (g o in_f' = f o in_f)
+       ==>
+       PSPEC ir (pre_p,post_p) stk_f (in_f', g, out_f)`,
+     RW_TAC std_ss [PSPEC_def, HSPEC_def] THEN
+     METIS_TAC [FUN_EQ_THM, combinTheory.o_THM]
+   );
+
+val PRJ_SC_RULE = Q.store_thm (
+   "PRJ_SC_RULE",
+   `!ir1 ir2 pre_p1 post_p1 post_p2 stk_f in_f1 f1 f2 out_f1 out_f2.
+     WELL_FORMED ir1 /\ WELL_FORMED ir2 /\
+     PSPEC ir1 (pre_p1,post_p1) stk_f (in_f1,f1,out_f1) /\ PSPEC ir2 (post_p1,post_p2) stk_f (out_f1,f2,out_f2) 
+       ==>
+       PSPEC (SC ir1 ir2) (pre_p1,post_p2) stk_f (in_f1,f2 o f1,out_f2)`,
 
      RW_TAC std_ss [PSPEC_def] THEN
      METIS_TAC [SC_RULE]
    );
 
-(*
-val PROJ_SC_RULE_2 = Q.store_thm (
-   "PROJ_SC_RULE_2",
-   `!ir1 ir2 f1 f2 in_f1 out_f1 in_f2 out_f2 convert_f.
-     WELL_FORMED ir1 /\ WELL_FORMED ir2 /\ (convert_f o out_f1 = in_f2) /\ 
-     PSPEC ir1 (pre_p1,post_p1) (in_f1,f1,out_f1) /\ PSPEC ir2 (post_p1,post_p2) (in_f2,f2,out_f2) 
-       ==>
-       PSPEC (SC ir1 ir2) (pre_p1,post_p2) (in_f1,f2 o convert_f o f1,out_f2)`,
-
-     RW_TAC std_ss [PSPEC_def, HSPEC_def] THEN
-     `!st. out_f2 (run_ir ir2 st) = (f2 o convert_f) (out_f1 st)` by RW_TAC std_ss [] THEN
-     POP_ASSUM MP_TAC THEN
-     POP_ASSUM (K ALL_TAC) THEN STRIP_TAC THEN
-     IMP_RES_TAC (SIMP_RULE std_ss [PSPEC_def, HSPEC_def] PROJ_SC_RULE) THEN
-     NTAC 14 (POP_ASSUM (K ALL_TAC)) THEN
-     METIS_TAC [combinTheory.o_THM]
-   );
-*)
-
-val PROJ_CJ_RULE = Q.store_thm (
-   "PROJ_CJ_RULE",
-   `!ir_t ir_f f1 f2 in_f out_f cond_f. 
+val PRJ_CJ_RULE = Q.store_thm (
+   "PRJ_CJ_RULE",
+   `!cond ir_t ir_f pre_p post_p stk_f cond_f in_f f1 f2 out_f. 
      WELL_FORMED ir_t /\ WELL_FORMED ir_f /\
-     PSPEC ir_t (pre_p,post_p) (in_f,f1,out_f) /\ PSPEC ir_f (pre_p, post_p) (in_f,f2,out_f) /\ (!st. cond_f (in_f st) = eval_cond cond st)
+     PSPEC ir_t (pre_p,post_p) stk_f (in_f,f1,out_f) /\ 
+     PSPEC ir_f (pre_p, post_p) stk_f (in_f,f2,out_f) /\ (!st. cond_f (in_f st) = eval_il_cond cond st)
         ==>
-       PSPEC (CJ cond ir_t ir_f) (pre_p,post_p) (in_f, (\v.if cond_f v then f1 v else f2 v), out_f)`,
+       PSPEC (CJ cond ir_t ir_f) (pre_p,post_p) stk_f (in_f, (\v.if cond_f v then f1 v else f2 v), out_f)`,
      
      RW_TAC std_ss [PSPEC_def, HSPEC_def] THEN
      METIS_TAC [IR_SEMANTICS_CJ]
    );
 
 (* Need the theorems in ARMCompositionTheory to prove the PROJ_TR_RULE *)
+val PRJ_TR_RULE = Q.store_thm (
+   "PRJ_TR_RULE",
+   `!cond ir pre_p stk_f cond_f prj_f f.
+        WELL_FORMED ir /\  WF (\st1 st0. ~eval_il_cond cond st0 /\ (st1 = run_ir ir st0)) /\
+        (!st. cond_f (prj_f st) = eval_il_cond cond st) /\ PSPEC ir (pre_p,pre_p) stk_f (prj_f,f,prj_f) ==> 
+          PSPEC (TR cond ir) (pre_p,pre_p) stk_f (prj_f, WHILE ($~ o cond_f) f, prj_f)`,
 
-(* 
-val PROJ_TR_RULE = Q.store_thm (
-   "PROJ_TR_RULE",
-   `!cond ir prj_f f cond_f.
-        WELL_FORMED ir /\  WF (\st1 st0. ~eval_cond cond st0 /\ (st1 = run_ir ir st0)) /\
-        (!st. cond_f (prj_f st) = eval_cond cond st) /\ PSPEC ir (pre_p,pre_p) (prj_f,f,prj_f) ==> 
-          PSPEC (TR cond ir) (pre_p,pre_p) (prj_f, WHILE ($~ o cond_f) f, prj_f)`,
+    RW_TAC std_ss [PSPEC_def] THEN 
+    RW_TAC std_ss [HSPEC_def] THENL [
+        FULL_SIMP_TAC std_ss [HSPEC_def] THEN
+            METIS_TAC [SIMP_RULE std_ss [HSPEC_def] TR_RULE, WF_TR_LEM_1],
 
-    RW_TAC std_ss [PSPEC_def, HSPEC_def] THEN
-    `WF_TR (cond,translate ir)` by METIS_TAC [WF_TR_LEM_1] THEN
-    FULL_SIMP_TAC std_ss [WELL_FORMED_def, run_ir_def, run_arm_def, translate_def] THEN
-    Q.ABBREV_TAC `arm = translate ir` THEN
-    IMP_RES_TAC (SIMP_RULE set_ss [] (Q.SPECL [`cond`,`arm`,`(\i. ARB)`,`(0,0w,st):STATE`,`{}`] ARMCompositionTheory.UNROLL_TR_LEM)) THEN
-    POP_ASSUM (ASSUME_TAC o Q.SPEC `st`) THEN
-    FULL_SIMP_TAC std_ss [FUNPOW, ARMCompositionTheory.get_st_def] THEN
-    NTAC 2 (POP_ASSUM (K ALL_TAC)) THEN
-    Induct_on `loopNum cond arm (\i.ARB) ((0,0w,st),{})` THENL [
-        REWRITE_TAC [Once EQ_SYM_EQ] THEN RW_TAC std_ss [FUNPOW,ARMCompositionTheory.get_st_def] THEN
-            IMP_RES_TAC ARMCompositionTheory.LOOPNUM_BASIC THEN
-            FULL_SIMP_TAC arith_ss [Once WHILE, ARMCompositionTheory.get_st_def],
+        IMP_RES_TAC (SIMP_RULE std_ss [PSPEC_def] PSPEC_STACK) THEN
+            POP_ASSUM (ASSUME_TAC o Q.SPEC `(stk_f:DSTATE->'a) st`) THEN
+            IMP_RES_TAC WF_TR_LEM_1 THEN
+            IMP_RES_TAC (Q.SPECL [`cond`,`ir`,`\st1. pre_p st1 /\ ((stk_f:DSTATE->'a) 
+			          st1 = (stk_f:DSTATE->'a) st)`] TR_RULE) THEN
+            POP_ASSUM (ASSUME_TAC o Q.SPEC `st` o SIMP_RULE std_ss [HSPEC_def]) THEN
+            METIS_TAC [],
 
-        REWRITE_TAC [Once EQ_SYM_EQ] THEN RW_TAC std_ss [FUNPOW] THEN
-            IMP_RES_TAC ARMCompositionTheory.LOOPNUM_INDUCTIVE THEN
-            `v = loopNum cond arm (\i.ARB) ((0,0w,SND (SND (FST (runTo (upload arm (\i.ARB) 0) (LENGTH arm) ((0,0w,st),{}))))),{})` by
-                METIS_TAC [ABS_PAIR_THM,DECIDE (Term`!x.0+x=x`),ARMCompositionTheory.LOOPNUM_INDEPENDENT_OF_CPSR_PCS, ARMCompositionTheory.get_st_def, 
-                        FST, SND, ARMCompositionTheory.DSTATE_IRRELEVANT_PCS,ARMCompositionTheory.well_formed_def] THEN
-            RES_TAC THEN Q.PAT_ASSUM `v = x` (ASSUME_TAC o GSYM) THEN FULL_SIMP_TAC std_ss [] THEN POP_ASSUM (K ALL_TAC) THEN
-            Q.PAT_ASSUM `v = x` (ASSUME_TAC o GSYM) THEN FULL_SIMP_TAC std_ss [] THEN POP_ASSUM (K ALL_TAC) THEN
-            Q.PAT_ASSUM `~x` (ASSUME_TAC o SIMP_RULE std_ss [ARMCompositionTheory.get_st_def]) THEN
-            RW_TAC std_ss [Once WHILE] THEN
-            Q.UNABBREV_TAC `arm` THEN
-            `run_ir ir st = SND (SND (FST (runTo (upload (translate ir) (\i. ARB) 0) (LENGTH (translate ir)) ((0,0w,st),{}))))` by RW_TAC arith_ss [
+        IMP_RES_TAC (SIMP_RULE std_ss [PSPEC_def] PSPEC_CHARACTERISTIC) THEN
+            Q.PAT_ASSUM `!v x.p` (K ALL_TAC) THEN
+            `WF_TR (translate_condition cond,translate ir)` by METIS_TAC [WF_TR_LEM_1] THEN
+	    FULL_SIMP_TAC std_ss [WELL_FORMED_def, HSPEC_def, run_ir_def, run_arm_def, translate_def, eval_il_cond_def] THEN
+	    Q.ABBREV_TAC `arm = translate ir` THEN
+	    IMP_RES_TAC (SIMP_RULE set_ss [] (Q.SPECL [`translate_condition cond`,`arm`,`(\i. ARB)`,`(0,0w,st):STATE`,`{}`] 
+                              ARMCompositionTheory.UNROLL_TR_LEM)) THEN
+	    POP_ASSUM (ASSUME_TAC o Q.SPEC `st`) THEN
+	    FULL_SIMP_TAC std_ss [FUNPOW, ARMCompositionTheory.get_st_def] THEN
+	    NTAC 2 (POP_ASSUM (K ALL_TAC)) THEN
+	    Induct_on `loopNum (translate_condition cond) arm (\i.ARB) ((0,0w,st),{})` THENL [
+	      REWRITE_TAC [Once EQ_SYM_EQ] THEN RW_TAC std_ss [FUNPOW,ARMCompositionTheory.get_st_def] THEN
+	      IMP_RES_TAC ARMCompositionTheory.LOOPNUM_BASIC THEN
+	      FULL_SIMP_TAC arith_ss [Once WHILE, ARMCompositionTheory.get_st_def],
+
+	    REWRITE_TAC [Once EQ_SYM_EQ] THEN RW_TAC std_ss [FUNPOW] THEN
+        IMP_RES_TAC ARMCompositionTheory.LOOPNUM_INDUCTIVE THEN
+	      `v = loopNum (translate_condition cond) arm (\i.ARB) ((0,0w,SND (SND (FST (runTo (upload arm (\i.ARB) 0) (LENGTH arm) 
+                   ((0,0w,st),{}))))),{})` by METIS_TAC [ABS_PAIR_THM,DECIDE (Term`!x.0+x=x`),
+                       ARMCompositionTheory.LOOPNUM_INDEPENDENT_OF_CPSR_PCS, ARMCompositionTheory.get_st_def, 
+                       FST, SND, ARMCompositionTheory.DSTATE_IRRELEVANT_PCS,ARMCompositionTheory.well_formed_def] THEN
+	      RES_TAC THEN Q.PAT_ASSUM `v = x` (ASSUME_TAC o GSYM) THEN 
+              FULL_SIMP_TAC std_ss [] THEN POP_ASSUM (K ALL_TAC) THEN
+	      Q.PAT_ASSUM `v = x` (ASSUME_TAC o GSYM) THEN FULL_SIMP_TAC std_ss [] THEN POP_ASSUM (K ALL_TAC) THEN
+	      Q.PAT_ASSUM `~x` (ASSUME_TAC o SIMP_RULE std_ss [ARMCompositionTheory.get_st_def]) THEN
+	      RW_TAC std_ss [Once WHILE] THEN
+	      Q.UNABBREV_TAC `arm` THEN
+	      `run_ir ir st = SND (SND (FST (runTo (upload (translate ir) (\i. ARB) 0) (LENGTH (translate ir)) 
+                  ((0,0w,st),{}))))` by RW_TAC arith_ss [
                    ARMCompositionTheory.get_st_def, run_ir_def, run_arm_def] THEN
-            METIS_TAC [SND,FST,ARMCompositionTheory.get_st_def,ARMCompositionTheory.FUNPOW_DSTATE, ABS_PAIR_THM]
-      ]
+	      METIS_TAC [SND,FST,ARMCompositionTheory.get_st_def,ARMCompositionTheory.FUNPOW_DSTATE, ABS_PAIR_THM]
+	    ]
+     ]
    );
 
-val PROJ_TR_RULE_2 = Q.store_thm (
-   "PROJ_TR_RULE_2",
-   `!cond ir prj_f f cond_f.
-        WELL_FORMED ir /\ (!st. cond_f (prj_f st) = eval_cond cond st) /\
+val PRJ_TR_RULE_2 = Q.store_thm (
+   "PRJ_TR_RULE_2",
+   `!cond ir stk_f cond_f prj_f f.
+        WELL_FORMED ir /\ (!st. cond_f (prj_f st) = eval_il_cond cond st) /\
         (?R. WF R /\ !t0 t1. ~cond_f t0 ==> R (f t0) t0) /\
-           PSPEC ir (prj_f,f,prj_f) ==> PSPEC (TR cond ir) (prj_f, WHILE ($~ o cond_f) f, prj_f)`,
+           PSPEC ir ((\st.T),(\st.T)) stk_f (prj_f,f,prj_f) ==> 
+		    PSPEC (TR cond ir) ((\st.T),(\st.T)) stk_f (prj_f, WHILE ($~ o cond_f) f, prj_f)`,
 
-    RW_TAC std_ss [PSPEC_def, HSPEC_def] THEN
-    `WF (\st1 st0. ~eval_cond cond st0 /\ (st1 = run_ir ir st0))` by METIS_TAC [WF_TR_LEM_2, WF_TR_LEM_3] THEN
-    METIS_TAC [SIMP_RULE std_ss [PSPEC_def, HSPEC_def] PROJ_TR_RULE]
+    SIMP_TAC std_ss [PSPEC_def, HSPEC_def] THEN
+    REPEAT GEN_TAC THEN NTAC 2 STRIP_TAC THEN
+    `WF (\st1 st0. ~eval_il_cond cond st0 /\ (st1 = run_ir ir st0))` by METIS_TAC [WF_TR_LEM_2, WF_TR_LEM_3] THEN
+    METIS_TAC [SIMP_RULE std_ss [PSPEC_def, HSPEC_def] (Q.SPECL [`cond`,`ir`,`\st.T`] PRJ_TR_RULE)]
   );
-*)
+
 
 (*---------------------------------------------------------------------------------*)
-(*      Rules for Context                                                          *) 
+(*      Rules for Conditions (projective function version)                         *) 
 (*---------------------------------------------------------------------------------*)
 
-val UNCHANGED_def = Define `
-    UNCHANGED ir contextL = 
-      !v. HSPEC (\st. MAP (mread st) contextL = v) ir (\st. MAP (mread st) contextL = v)`;
-
-val CONTEXT_TR_RULE = Q.store_thm (
-   "CONTEXT_TR_RULE",
-   `!cond ir contextL.
-        WELL_FORMED ir /\  WF (\st1 st0. ~eval_cond cond st0 /\ (st1 = run_ir ir st0)) /\
-           UNCHANGED ir contextL ==> UNCHANGED (TR cond ir) contextL`,
-
-    RW_TAC std_ss [UNCHANGED_def] THEN 
-    METIS_TAC [TR_RULE, WF_TR_LEM_1]
+val PRJ_STRENGTHEN_RULE = Q.store_thm (
+   "PRJ_STRENGTHEN_RULE",
+   `!ir pre_p pre_p' post_p stk_f in_f f out_f.
+     WELL_FORMED ir /\
+     PSPEC ir (pre_p,post_p) stk_f (in_f,f,out_f) /\ (!st. pre_p' st ==> pre_p st) ==>
+       PSPEC ir (pre_p',post_p) stk_f (in_f,f,out_f)`,
+     RW_TAC std_ss [PSPEC_def, HSPEC_def]
    );
 
-val CONTEXT_SC_RULE = Q.store_thm (
-   "CONTEXT_SC_RULE",
-   `!ir1 ir2 contextL.
-        WELL_FORMED ir1 /\  WELL_FORMED ir2  /\ 
-        UNCHANGED ir1 contextL /\ UNCHANGED ir2 contextL 
-          ==> UNCHANGED (SC ir1 ir2) contextL`,
-
-    RW_TAC std_ss [UNCHANGED_def] THEN 
-    METIS_TAC [SC_RULE]
-   );
-
-val CONTEXT_CJ_RULE = Q.store_thm (
-   "CONTEXT_CJ_RULE",
-   `!ir1 ir2 cond contextL.
-        WELL_FORMED ir1 /\  WELL_FORMED ir2  /\ 
-        UNCHANGED ir1 contextL /\ UNCHANGED ir2 contextL 
-          ==> UNCHANGED (CJ cond ir1 ir2) contextL`,
-
-    RW_TAC std_ss [UNCHANGED_def] THEN
-    METIS_TAC [CJ_RULE_2]
+val PRJ_WEAKEN_RULE = Q.store_thm (
+   "PRJ_WEAKEN_RULE",
+   `!ir pre_p post_p post_p' stk_f in_f f out_f.
+     WELL_FORMED ir /\
+     PSPEC ir (pre_p,post_p) stk_f (in_f,f,out_f) /\ (!st. post_p st ==> post_p' st) ==>
+       PSPEC ir (pre_p,post_p') stk_f (in_f,f,out_f)`,
+     RW_TAC std_ss [PSPEC_def, HSPEC_def]
    );
 
 (*---------------------------------------------------------------------------------*)
-(*      Rules for Well-formedness                                    *) 
+(*      Rules for Stack (projective function version)                              *) 
+(*---------------------------------------------------------------------------------*)
+
+val valid_push_def = Define `
+    valid_push (stk_f,in_f,f,out_f) (stk_f',in_f',g,out_f') =
+      !st st'. (stk_f st' = stk_f st) /\ (out_f st' = f (in_f st)) ==>
+         (stk_f' st' = stk_f' st) /\ (out_f' st' = g (in_f' st))`;
+
+val PRJ_POP_RULE = Q.store_thm (
+   "PRJ_POP_RULE",
+   `!ir pre_p post_p stk_f in_f f out_f stk_f' in_f' g out_f'.
+      PSPEC ir (pre_p,post_p) stk_f (in_f,f,out_f) /\ 
+	valid_push (stk_f,in_f,f,out_f) (stk_f',in_f',g,out_f')
+       ==>
+        PSPEC ir (pre_p,post_p) stk_f' (in_f', g, out_f')`,
+    RW_TAC list_ss [PSPEC_def, HSPEC_def, valid_push_def]
+   );
+
+val P_intact_def = Define `
+    P_intact (P,Q) (stk_f,stk_g) =
+     !st st'. (stk_f st' = stk_f st) /\ P st /\ Q st'
+           ==> (stk_g st' = stk_g st)`;
+
+val PRJ_PUSH_RULE = Q.store_thm (
+   "PRJ_PUSH_RULE",
+   `!ir pre_p post_p stk_f in_f f out_f e_f stk_g.
+      PSPEC ir (pre_p,post_p) stk_f (in_f,f,out_f) /\ 
+        P_intact (pre_p,post_p) (stk_f,stk_g)  
+      ==> PSPEC ir (pre_p,post_p) stk_g (in_f, f, out_f)`,
+    RW_TAC list_ss [PSPEC_def, HSPEC_def, P_intact_def]
+   );
+
+(*---------------------------------------------------------------------------------*)
+(*      Hoare Rules on Projection on Inputs and Ouputs (represented by vectors)    *)
+(*      To overcome the type restriction on tuples in HOL definitions              *)
+(*---------------------------------------------------------------------------------*)
+
+(*   Vectors *)
+
+val _ = Hol_datatype `
+    VEXP = SG of DATA                (* registers *)
+         | VT of VEXP # VEXP         (* pairs     *)
+    `;
+
+val readv_def = Define ` 
+    (readv st (PR (a,b)) = VT (readv st a, readv st b)) /\
+    (readv st x = SG (read st (toEXP x)))`;
+
+(* Vector Stack, modelled as a list of expression vectors *)
+
+val push_def = Define `
+    push x stk = x :: stk`;
+
+val top_def = Define `
+    top  = HD`;
+
+val pop_def = Define `
+    pop  = TL`;
+
+(* Specification on vectors *)
+
+val VSPEC_def = Define `
+    VSPEC ir (pre_p,post_p) stk (iv,f,ov) = 
+        PSPEC ir (pre_p,post_p) (\st. MAP (readv st) stk) ((\st.readv st iv), f, (\st.readv st ov))
+    `;
+
+val _ = type_abbrev("VSPEC_TYPE", type_of (Term `VSPEC`));
+
+val V_SHUFFLE_RULE = Q.store_thm (
+   "V_SHUFFLE_RULE",
+   `!ir stk iv f ov g iv'.
+     VSPEC ir (pre_p,post_p) stk (iv,f,ov) /\ (!st. g (readv st iv') = f (readv st iv))
+       ==>
+       VSPEC ir (pre_p,post_p) stk (iv', g, ov)`,
+     RW_TAC std_ss [VSPEC_def, PSPEC_def, HSPEC_def]
+   );
+
+val V_SC_RULE = Q.store_thm (
+   "V_SC_RULE",
+   `!ir1 ir2 pre_p1 post_p1 post_p2 stk vi1 f1 vo1 f2 vo2.
+     WELL_FORMED ir1 /\ WELL_FORMED ir2 /\
+     VSPEC ir1 (pre_p1,post_p1) stk (vi1,f1,vo1) /\ VSPEC ir2 (post_p1,post_p2) stk (vo1,f2,vo2) 
+       ==>
+       VSPEC (SC ir1 ir2) (pre_p1,post_p2) stk (vi1,f2 o f1,vo2)`,
+     RW_TAC std_ss [VSPEC_def] THEN
+     METIS_TAC [PRJ_SC_RULE]
+   );
+
+val V_CJ_RULE = Q.store_thm (
+   "V_CJ_RULE",
+   `!cond ir_t ir_f pre_p post_p stk cond_f iv f1 f2 ov. 
+     WELL_FORMED ir_t /\ WELL_FORMED ir_f /\
+     VSPEC ir_t (pre_p,post_p) stk (iv,f1,ov) /\ 
+     VSPEC ir_f (pre_p, post_p) stk (iv,f2,ov) /\ (!st. cond_f (readv st iv) = eval_il_cond cond st)
+        ==>
+       VSPEC (CJ cond ir_t ir_f) (pre_p,post_p) stk (iv, (\v.if cond_f v then f1 v else f2 v), ov)`,
+     RW_TAC std_ss [VSPEC_def] THEN
+     FULL_SIMP_TAC std_ss [PRJ_CJ_RULE]
+   );
+
+(* Need the theorems in ARMCompositionTheory to prove the PROJ_TR_RULE *)
+
+val V_TR_RULE = Q.store_thm (
+   "V_TR_RULE",
+   `!cond ir pre_p stk cond_f iv f.
+        WELL_FORMED ir /\  WF (\st1 st0. ~eval_il_cond cond st0 /\ (st1 = run_ir ir st0)) /\
+        (!st. cond_f (readv st iv) = eval_il_cond cond st) /\ VSPEC ir (pre_p,pre_p) stk (iv,f,iv) ==> 
+          VSPEC (TR cond ir) (pre_p,pre_p) stk (iv, WHILE ($~ o cond_f) f, iv)`,
+
+    RW_TAC std_ss [VSPEC_def] THEN 
+    FULL_SIMP_TAC std_ss [PRJ_TR_RULE]
+   );
+
+(*---------------------------------------------------------------------------------*)
+(*      Rules for Conditions (vector version)                                      *) 
+(*---------------------------------------------------------------------------------*)
+
+val V_STRENGTHEN_RULE = Q.store_thm (
+   "V_STRENGTHEN_RULE",
+   `!ir pre_p pre_p' post_p stk iv f ov.
+     WELL_FORMED ir /\
+     VSPEC ir (pre_p,post_p) stk (iv,f,ov) /\ (!st. pre_p' st ==> pre_p st) ==>
+       VSPEC ir (pre_p',post_p) stk (iv,f,ov)`,
+     RW_TAC std_ss [VSPEC_def] THEN
+     METIS_TAC [PRJ_STRENGTHEN_RULE]
+   );
+
+val V_WEAKEN_RULE = Q.store_thm (
+   "V_WEAKEN_RULE",
+   `!ir pre_p post_p post_p' stk iv f ov.
+     WELL_FORMED ir /\
+     PSPEC ir (pre_p,post_p) stk (iv,f,ov) /\ (!st. post_p st ==> post_p' st) ==>
+       PSPEC ir (pre_p,post_p') stk (iv,f,ov)`,
+     RW_TAC std_ss [VSPEC_def] THEN
+     METIS_TAC [PRJ_WEAKEN_RULE]
+   );
+
+(*---------------------------------------------------------------------------------*)
+(*      Rules for Stack (vector version)                                           *) 
+(*---------------------------------------------------------------------------------*)
+
+val V_POP_RULE = Q.store_thm (
+   "V_POP_RULE",
+   `!ir pre_p post_p stk iv f ov e g.
+      VSPEC ir (pre_p,post_p) (e::stk) (iv,f,ov) /\ 
+       (!st. g (readv st (PR(iv,e))) = VT (f (readv st iv), readv st e)) ==>
+         VSPEC ir (pre_p,post_p) stk (PR(iv,e), g, PR(ov,e))`,
+    RW_TAC list_ss [VSPEC_def, PSPEC_def, HSPEC_def, readv_def]
+   );
+
+val V_intact_def = Define `
+    V_intact (P,Q,e) =
+      ?x. (!st.P st ==> (readv st e = x)) /\ (!st.Q st ==> (readv st e = x))`;
+
+
+val V_PUSH_RULE = Q.store_thm (
+   "V_PUSH_RULE",
+   `!ir pre_p post_p stk iv f ov e.
+      VSPEC ir (pre_p,post_p) stk (iv,f,ov) /\ V_intact(pre_p, post_p, e)  
+      ==>
+         VSPEC ir (pre_p,post_p) (e::stk) (iv, f, ov)`,
+    RW_TAC list_ss [VSPEC_def, PSPEC_def, HSPEC_def, V_intact_def, readv_def] THEN
+    METIS_TAC []
+   );
+
+
+(*---------------------------------------------------------------------------------*)
+(*      Rules for Well-formedness                                                  *) 
 (*---------------------------------------------------------------------------------*)
 
 val WELL_FORMED_TR_RULE = Q.store_thm (
    "WELL_FORMED_TR_RULE",
    `!cond ir context_f.
-        WELL_FORMED ir /\  WF (\st1 st0. ~eval_cond cond st0 /\ (st1 = run_ir ir st0)) ==>
+        WELL_FORMED ir /\  WF (\st1 st0. ~eval_il_cond cond st0 /\ (st1 = run_ir ir st0)) ==>
            WELL_FORMED (TR cond ir)`,
 
     RW_TAC std_ss [] THEN 
@@ -394,4 +615,3 @@ val WELL_FORMED_TR_RULE = Q.store_thm (
    );
 
 val _ = export_theory();
-
