examples/dev/sw/examples/simple_examples.sml
@@ -1,0 +1,264 @@
+(*---------------------------------------------------------------------------------*)
+(*      Simple Examples                                                            *) 
+(*      No precedure call is presented in these examples                           *)
+(*---------------------------------------------------------------------------------*)
+val hol_dir = "/home/tt291/hol98/";
+loadPath := (concat hol_dir "examples/dev/sw") :: 
+            !loadPath;
+
+use (concat hol_dir "examples/dev/sw/compiler");
+
+(*---------------------------------------------------------------------------------*)
+(*      Single Blocks                                                              *)
+(*      The ShiftXor procedure appearing in TEA                                    *)
+(*---------------------------------------------------------------------------------*)
+
+val ShiftXor_def =
+ Define
+   `ShiftXor (x:word32,s,k0,k1) = ((x << 4) + k0) ?? (x + s) ?? ((x >> 5) + k1)`;
+
+(*
+- val spec = pp_compile ShiftXor_def;
+|- !st.
+          get_st
+            (run_arm
+               [((LSL,NONE,F),SOME (REG 4),[REG 0; WCONST 4w],NONE);
+                ((ADD,NONE,F),SOME (REG 2),[REG 4; REG 2],NONE);
+                ((ADD,NONE,F),SOME (REG 1),[REG 0; REG 1],NONE);
+                ((EOR,NONE,F),SOME (REG 1),[REG 2; REG 1],NONE);
+                ((ASR,NONE,F),SOME (REG 0),[REG 0; WCONST 5w],NONE);
+                ((ADD,NONE,F),SOME (REG 0),[REG 0; REG 3],NONE);
+                ((EOR,NONE,F),SOME (REG 0),[REG 1; REG 0],NONE)]
+               ((0,0w,st),{}))<MR R0> =
+          ShiftXor (st<MR R0>,st<MR R1>,st<MR R2>,st<MR R3>))
+
+- extract_arm spec;
+  Name              : ShiftXor
+  Arguments         : (r0,(r1,(r2,r3)))
+  Returns           : r0
+  Body: 
+    0:          lsl     r4, r0, #4iw
+    1:          add     r2, r4, r2
+    2:          add     r1, r0, r1
+    3:          eor     r1, r2, r1
+    4:          asr     r0, r0, #5iw
+    5:          add     r0, r0, r3
+    6:          eor     r0, r1, r0
+
+*)
+
+(*---------------------------------------------------------------------------------*)
+(*      Single Conditional Jump                                                    *)
+(*      "let" statements are supported                                             *)
+(*---------------------------------------------------------------------------------*)
+
+val cj_f_1_def = Define `
+    cj_f_1 (a,b:word32) = 
+       if a = 1w then 
+            let e = a + b + 3w
+            in e 
+       else let c = a + b in 
+            let d = c * c - a in
+            d`;
+
+(*
+- val spec = pp_compile cj_f_1_def;
+...
+|- !st.
+          get_st
+            (run_arm
+               [((CMP,NONE,F),NONE,[REG 0; WCONST 1w],NONE);
+                ((B,SOME EQ,F),NONE,[],SOME (POS 5));
+                ((ADD,NONE,F),SOME (REG 1),[REG 0; REG 1],NONE);
+                ((MUL,NONE,F),SOME (REG 1),[REG 1; REG 1],NONE);
+                ((SUB,NONE,F),SOME (REG 0),[REG 1; REG 0],NONE);
+                ((B,SOME AL,F),NONE,[],SOME (POS 3));
+                ((ADD,NONE,F),SOME (REG 0),[REG 0; REG 1],NONE);
+                ((ADD,NONE,F),SOME (REG 0),[REG 0; WCONST 3w],NONE)]
+               ((0,0w,st),{}))<MR R0> =
+          cj_f_1 (st<MR R0>,st<MR R1>))
+
+- extract_ir spec;
+  Name              : cj_f_1
+  Arguments         : (r0,r1)
+  Returns           : r0
+  Body: 
+  CJ(r0 = #1w,
+    [madd r0 r0 r1; madd r0 r0 #3w],
+    [madd r1 r0 r1; mmul r1 r1 r1; msub r0 r1 r0])
+
+- extract_arm spec;
+
+  Name              : cj_f_1
+  Arguments         : (r0,r1)
+  Returns           : r0
+  Body: 
+    0:          cmp     r0, #1iw
+    1:          beq     + (5)
+    2:          add     r1, r0, r1
+    3:          mul     r1, r1, r1
+    4:          sub     r0, r1, r0
+    5:          bal     + (3)
+    6:          add     r0, r0, r1
+    7:          add     r0, r0, #3iw
+*)
+
+(*---------------------------------------------------------------------------------*)
+(*      Tail Recusive Functions                                                    *)
+(*      Factorial Function. Form: SC (TR, BLK)                                     *) 
+(*      This is the example 1 in the paper                                         *)
+(*---------------------------------------------------------------------------------*)
+val WORD_LO___MEASURE = store_thm ("WORD_LO___MEASURE",
+  ``word_lo = measure w2n``,
+  SIMP_TAC std_ss [FUN_EQ_THM, prim_recTheory.measure_def,
+    relationTheory.inv_image_def, WORD_LO] );
+
+val fact_def = Hol_defn "fact" 
+   `fact (x:word32,a:word32) = if x=0w then a else fact(x-1w, x*a)`;
+
+val (fact_def, fact_ind) =
+Defn.tprove (fact_def,
+  TotalDefn.WF_REL_TAC `inv_image $<+ (\(v1:word32,v2:word32). v1)` THENL [
+    SIMP_TAC std_ss [WORD_LO___MEASURE, prim_recTheory.WF_measure],
+    SIMP_TAC std_ss [WORD_LO, WORD_PRED_THM]
+  ])
+
+val fact_thm = Q.store_thm (
+   "fact_thm",
+   `fact = (\(x,a).a) o (WHILE ($~ o (\(x,a).x = 0w)) (\(x,a).(x-1w,x*a)))`,
+   SIMP_TAC std_ss [FUN_EQ_THM, FORALL_PROD] THEN
+   HO_MATCH_MP_TAC fact_ind THEN
+   REPEAT STRIP_TAC THEN
+   ONCE_REWRITE_TAC [fact_def, WHILE] THEN
+   RW_TAC std_ss []
+  );
+
+
+(*
+-   extra_defs := [fact_thm];
+-   pp_compile fact_def;
+
+   |- !st.
+         get_st
+           (run_arm
+              [((CMP,NONE,F),NONE,[REG 0; WCONST 0w],NONE);
+               ((B,SOME EQ,F),NONE,[],SOME (POS 6));
+               ((SUB,NONE,F),SOME (REG 3),[REG 0; WCONST 1w],NONE);
+               ((MUL,NONE,F),SOME (REG 2),[REG 0; REG 1],NONE);
+               ((MOV,NONE,F),SOME (REG 0),[REG 3],NONE);
+               ((MOV,NONE,F),SOME (REG 1),[REG 2],NONE);
+               ((B,SOME AL,F),NONE,[],SOME (NEG 6));
+               ((MOV,NONE,F),SOME (REG 2),[REG 1],NONE)]
+              ((0,0w,st),{}))<MR R2> =
+         fact (st<MR R0>,st<MR R1>) 
+
+
+*)
+
+(*---------------------------------------------------------------------------------*)
+(*      Constants are replaced by simpler ones that can be represented             *)
+(*---------------------------------------------------------------------------------*)
+
+val const_1_def = Define `
+    const_1 (x:word32) = (x + 0xFF0012Fw) - 0x1003w`;
+
+pp_compile const_1_def;
+
+
+(*---------------------------------------------------------------------------------*)
+(*      before that a evaluation takes place                                       *)
+(*---------------------------------------------------------------------------------*)
+
+val const_2_def = Define `
+    const_2 (x:word32) = (x + (0xFF0012Fw - 0x1003w))`;
+
+pp_compile const_2_def;
+
+
+(*---------------------------------------------------------------------------------*)
+(*      commutativity is exploited                                                 *)
+(*---------------------------------------------------------------------------------*)
+
+val const_3_def = Define `
+    const_3 (x:word32) = (1w + x)`;
+
+pp_compile const_3_def;
+
+
+(*---------------------------------------------------------------------------------*)
+(*      multiplication examples                                                    *)
+(*         no constants                                                            *)
+(*         modified register allocation                                            *)
+(*---------------------------------------------------------------------------------*)
+
+val mul_1_def = Define `
+    mul_1 (x:word32) = (x * 2w)`;
+
+pp_compile mul_1_def;
+
+val mul_2_def = Define `
+    mul_2 (x:word32) = (x * x)`;
+
+pp_compile mul_2_def;
+
+(*---------------------------------------------------------------------------------*)
+(*      Composition of various structures                                          *)
+(*      "Let" statement is allowed                                                 *)
+(*      This example has the form SC (BLK, CJ)                                     *)
+(*      This is the example 2 in the paper                                         *)
+(*---------------------------------------------------------------------------------*)
+
+val cj_f_2_def = Define `
+    cj_f_2 (a:word32,b:word32) = let c = a + 1w in
+               if a = 1w then c else c + b`;
+
+(*
+pp_compile cj_f_2_def;
+
+ |- !st.
+          get_st
+            (run_arm
+               [((ADD,NONE,F),SOME (REG 2),[REG 0; WCONST 1w],NONE);
+                ((CMP,NONE,F),NONE,[REG 0; WCONST 1w],NONE);
+                ((B,SOME EQ,F),NONE,[],SOME (POS 3));
+                ((ADD,NONE,F),SOME (REG 2),[REG 2; REG 1],NONE);
+                ((B,SOME AL,F),NONE,[],SOME (POS 1))]
+               ((0,0w,st),{}))<MR R2> =
+          cj_f_2 (st<MR R0>,st<MR R1>))
+
+  Name              : cj_f_2
+  Arguments         : (r0,r1)
+  Returns           : r2
+  Body: 
+    0:          add     r2, r0, #1iw
+    1:          cmp     r0, #1iw
+    2:          beq     + (3)
+    3:          add     r2, r2, r1
+    4:          bal     + (1)
+*)
+
+
+(*---------------------------------------------------------------------------------*)
+(*      This example encounters a bug in the front end (CPS conversion)            *)
+(*---------------------------------------------------------------------------------*)
+
+(* A more complicated SC example.  Form: SC (BLK, SC (CJ, BLK))         *)
+(* The ANF conversion seems wrong ???                                   *)
+
+val f3_def = Define `
+    f3 (a:word32,b:word32) = let c = a + 1w in
+               let d = if a = 1w then b else a + b in
+               let e = c - d in
+               e 
+`;
+
+pp_compile ((SIMP_RULE std_ss [LET_THM]) f3_def)
+toANF [] f3_def
+(*
+*)
+
+
+(*---------------------------------------------------------------------------------*)
+(*      See the "fc_examples.sml" for examples involving function calls            *)
+(*---------------------------------------------------------------------------------*)
+
